Travail accompli jusqu'au 26 mai

tre_completeness_src.v
@@ -5,8 +5,10 @@ Import ListNotations.
 
 Inductive form :=
   | Atome : nat -> form
-  | And : form -> form -> form
+  | And : form -> form -> form.
+  (*
   | Or : form -> form -> form.
+  *)
 
 (*
 Fixpoint sem (M : nat -> Prop) (A : form) :=
@@ -24,22 +26,33 @@ Inductive included : context -> context -> Prop :=
   | included_cons_no : forall A ctx ctx', included ctx ctx' -> included ctx (cons A ctx')
   | included_cons_yes : forall A ctx ctx', included ctx ctx' -> included (cons A ctx) (cons A ctx').
 
+Definition extend (ctx ctx' : context) := included ctx' ctx.
+
 Inductive In (A : form) : context -> Prop :=
   | In_cons_yes : forall ctx, In A (cons A ctx)
   | In_cons_no : forall ctx, In A ctx -> forall B, In A (cons B ctx).
 
 Inductive provable : context -> form -> Prop :=
-  | Ax ctx A : In A ctx -> provable ctx A
-  | AndI ctx A B : provable ctx A -> provable ctx B -> provable ctx (And A B)
-  | AndE1 ctx A B : provable ctx (And A B) -> provable ctx A
-  | AndE2 ctx A B : provable ctx (And A B) -> provable ctx B
+  | Ax { ctx A } : In A ctx -> provable ctx A
+  | AndI { ctx A B } : provable ctx A -> provable ctx B -> provable ctx (And A B)
+  | AndE1 { ctx A B } : provable ctx (And A B) -> provable ctx A
+  | AndE2 { ctx A B } : provable ctx (And A B) -> provable ctx B.
+  (*
   | OrI1 ctx A B : provable ctx A -> provable ctx (Or A B)
   | OrI2 ctx A B : provable ctx B -> provable ctx (Or A B)
   | OrE ctx A B : forall C, provable ctx (Or A B) -> provable (cons A ctx) C -> provable (cons B ctx) C -> provable ctx C.
+  *)
+
+Fixpoint semK (K : context -> nat -> Prop) (ctx : context) (A : form) :=
+  match A with
+    | Atome n   => K ctx n 
+    | And A1 A2 => ((semK K ctx A1) * (semK K ctx A2))%type
+    (*| Or A1 A2  => (semK K ctx A1) \/ (semK K ctx A2)*)
+  end.
 
 (*Definition valid M A := forall (M : nat -> Prop) (A : form), sem M A.*)
 
-Notation "p 'INCL' q" := (forall R, included p R -> included q R) (at level 70, q at next level).
+Notation "p 'INCL' q" := (forall R, extend p R -> extend q R) (at level 70, q at next level).
 Notation "'forallI' q 'INCL' p , P" := (forall q, q INCL p -> P q) (at level 200, q at level 69, p at level 69).
 
 Lemma refl_incl :
@@ -54,39 +67,166 @@ Proof.
   auto.
 Defined.
 
-Forcing Translate nat using context included.
-Forcing Translate form using context included.
+Forcing Translate nat using context extend.
+Forcing Translate form using context extend.
 
-Forcing Definition sem : forall (M : nat -> Prop) (A : form), Prop using context included.
+Forcing Definition sem : forall (M : nat -> Prop) (A : form), Prop using context extend.
 Proof.
   exact (fun p M A p0 Hincl => (* Hincl : preuve de p0 INCL p *)
     (fix sem p1 Hincl1 A := (* Hincl1 : preuve de p1 INCL p *)
       match A with
       | Atomeᶠ _ n   => M p1 Hincl1 n p1 (refl_incl p1)
       | Andᶠ _ A1 A2 => (sem p1 Hincl1 (A1 p1 (refl_incl p1))) /\ (sem p1 Hincl1 (A2 p1 (refl_incl p1)))
-      | Orᶠ _ A1 A2  => (sem p1 Hincl1 (A1 p1 (refl_incl p1))) \/ (sem p1 Hincl1 (A2 p1 (refl_incl p1)))
+      (*| Orᶠ _ A1 A2  => (sem p1 Hincl1 (A1 p1 (refl_incl p1))) \/ (sem p1 Hincl1 (A2 p1 (refl_incl p1)))*)
     end) p (refl_incl p) (A p (refl_incl p)) 
   ).
 Defined.
 
+Print natᶠ.
+
 Definition valid A := forall (M : nat -> Prop), sem M A.
-Forcing Translate valid using context included.
+Forcing Translate valid using context extend.
 
-Forcing Translate list using context included.
-Forcing Translate context using context included.
+Forcing Translate list using context extend.
+Forcing Translate context using context extend.
 
-Forcing Translate In using context included.
-Forcing Translate provable using context included.
+Forcing Translate In using context extend.
+Forcing Translate provable using context extend.
 
-Axiom psi : forall { p }, formᶠ p -> form.
+Lemma psi_nat : forall { p }, (forallI p0 INCL p, natᶠ) -> nat.
+Proof.
+  exact (fun p n =>
+    (fix psi_nat_rec n := 
+      match n with 
+      | Oᶠ _    => O 
+      | Sᶠ _ m  => S (psi_nat_rec (m p (refl_incl p)))
+      end 
+    ) (n p (refl_incl p)) 
+  ).
+Qed.
+
+Lemma phi_nat : forall (p : context), nat -> natᶠ p.
+Proof.
+  exact (fun p n =>
+    (fix phi_nat_rec p n :=
+      match n with 
+      | O => Oᶠ p
+      | S m => Sᶠ p (fun p0 Hp0 => (phi_nat_rec p0 m))
+      end 
+    ) p n 
+  ).
+Qed.
+
+Lemma psi_form : forall { p }, (forallI p0 INCL p, formᶠ) -> form.
+Proof.
+  exact (fun p A =>
+    (fix psi_rec A := 
+      match A with 
+      | Atomeᶠ _ n    => Atome (psi_nat n) 
+      | Andᶠ _ A1 A2  => And (psi_rec (A1 p (refl_incl p))) (psi_rec (A2 p (refl_incl p)))
+      (*| Orᶠ _ A1 A2   => Or (psi_rec (A1 p (refl_incl p))) (psi_rec (A2 p (refl_incl p)))*)
+      end) (A p (refl_incl p)) 
+  ).
+Defined.
+
+Lemma phi_form : forall { p }, form -> formᶠ p.
+Proof.
+  exact (fun p A => 
+    (fix phi_form_rec p A :=
+      match A with 
+      | Atome n => Atomeᶠ p (fun p0 _ => phi_nat p0 n)
+      | And A1 A2 => Andᶠ p (fun p0 _ => phi_form_rec p0 A1) (fun p0 _ => phi_form_rec p0 A2) 
+      end) p A 
+  ).
+Defined.
+
+Lemma id_form : forall { p } A, phi_form (psi_form A) = A p (refl_incl p).
+Proof.
+Admitted.
+
+Print provableᶠ.
+
+(*Lemma psi_provable : forall p M A, provableᶠ p M A -> provable (M) (psi_form (A p (refl_incl p))).
+Proof.
+  exact (fun p M A prov =>
+    (fix psi_prov_rec prov :=
+      match prov with
+      | Axᶠ
+    )
+  ).
+Admitted.*)
+
+(* Modèle universel *)
+Definition K0 ctx n := provable ctx (Atome n).
+
+Fixpoint reify p A : semK K0 p A -> provable p A :=
+  match A with 
+    | Atome n   => (fun v => v)
+    | And A1 A2 => (fun '(v1, v2) => AndI (reify p A1 v1) (reify p A2 v2))
+  end 
+with reflect p A : provable p A -> semK K0 p A :=
+  match A with 
+    | Atome n   => (fun t => t)
+    | And A1 A2 => (fun t => (reflect p A1 (AndE1 t), reflect p A2 (AndE2 t)))
+  end.
+
+Print contextᶠ.
+
+Lemma psi_model : forall { p : context } (M : forall p0 : context, p0 INCL p ->
+  (forallI p1 INCL p0, natᶠ) -> forall p1 : context, p1 INCL p0 -> Prop), context -> nat -> Prop.
+Proof.
+  exact (fun p M ctx n => M p (refl_incl p) (fun p0 _ => (phi_nat p0 n)) p (refl_incl p)).
+Qed.
+
+Lemma phi_model : forall (M : context -> nat -> Prop), 
+  forall { p : context }, forall p0 : context, p0 INCL p ->
+    (forallI p1 INCL p0, natᶠ) -> forall p1 : context, p1 INCL p0 -> Prop.
+Proof.
+  exact (fun M p (p0 : context) Hinclp0 (n : forallI p INCL p0, natᶠ) p1 Hinclp1 
+      => M p1 (psi_nat n) ).
+Qed.
+
+(*Axiom psi_sem : forall { p M A p0 Hinclp0 }, semᶠ p (phi_model M) (fun p1 _ => phi_form A) p0 Hinclp0 -> semK M p A.*)
+Axiom psi_sem : forall { p M A p0 Hinclp0 }, semᶠ p (phi_model M) A p0 Hinclp0 -> semK M nil (psi_form A).
+
+Lemma phi_context : forall { p }, context -> contextᶠ p p (refl_incl p).
+Proof.
+  exact (fun p ctx =>
+    (fix phi_ctx_rec p ctx : contextᶠ p p (refl_incl p) :=
+      match ctx with 
+      | [] => nilᶠ p _
+      | A :: ctx' => consᶠ p _ (fun p1 _ => phi_form A) (fun p1 _ => phi_ctx_rec p1 ctx')
+      end 
+    ) p ctx
+  ).
+Defined.
+
+Lemma phi_provable : forall { p ctx A }, provable ctx (psi_form A) -> provableᶠ p (fun p0 Hincl => (phi_context ctx) ) A.
+Proof.
+  intros. inversion_clear H.
+  - apply Axᶠ. intros. induction H0.
+    * simpl. Set Printing All. apply (In_cons_yesᶠ p0 (fun (p : context) (α0 : p INCL p0) =>
+    A p (fun (R : context) (k : extend p R) => α R (α0 R k)))). 
+Admitted.
+
 
 (*Forcing Translate and using context included.*)
-Forcing Definition completeness : forall A, valid A -> provable nil A using context included.
+Forcing Definition completeness : forall A, valid A -> provable nil A using context extend.
 Proof.
   intros. 
 
   specialize H with (p0 := p) (α := refl_incl p). simpl in H. fold (refl_incl p) in H.
   unfold refl_incl at 1 in H. unfold validᶠ in H.
-  specialize H with (M := fun (p0 : context) Hinclp0 (n : forallI p INCL p0, natᶠ) p1 Hinclp1 => provable p1 (psi (A p1 (trans_incl Hinclp1 Hinclp0))) ).
+  specialize H with (M := phi_model K0). 
 
   simpl.
+
+  apply psi_sem in H . apply reify in H.
+  change (provableᶠ p
+    (fun (p0 : context) (_ : p0 INCL p) =>
+     nilᶠ p0
+       (fun (p1 : context) (_ : p1 INCL p0) (p2 : context) (_ : p2 INCL p1) =>
+        formᶠ p2))
+      A
+  ).
+  change (provable nil (psi_form A)) in H.
